Minor Changes

CompCert/cfrontend/MoSel.v
@@ -1,10 +1,10 @@
 From iris.proofmode Require Export base intro_patterns spec_patterns
-                                   sel_patterns coq_tactics reduction
-                                   coq_tactics ltac_tactics.
+     sel_patterns coq_tactics reduction
+     coq_tactics ltac_tactics.
 Require Import FunctionalExtensionality.
 From iris Require Export bi.bi proofmode.tactics proofmode.monpred proofmode.reduction.
 From stdpp Require Export pmap.
-Require Import Ctypes.
+
 Axiom prop_extensionality : forall A B:Prop, (A <-> B) -> A = B.
 Global Set Warnings "-convert_concl_no_check".
 
@@ -17,79 +17,436 @@ Definition pred_impl {A} (P Q : A -> Prop) :=
 Notation "P ==> Q" := (pred_incl P Q).
 
 Module SepBasicCore.
+  Export monpred.
+  Section hprop.
+    Context {type : Type}.
+    Definition heap : Type := Pmap type.
 
-  Definition heap : Type := Pmap type.
+    (* Properties on heap *)
+    Instance heap_union_empty_l : LeftId (=@{heap}) ∅ (∪) := _.
+    Instance heap_union_empty_r : RightId (=@{heap}) ∅ (∪) := _.
+    Instance heap_union_assoc : base.Assoc (=@{heap}) (∪).
+    Proof.
+      intros m1 m2 m3. unfold base.union, map_union, union_with, map_union_with.
+      apply (merge_assoc _). intros i.
+      unfold heap in m1. unfold heap in m2. unfold heap in m3.
+        by destruct (m1 !! i), (m2 !! i), (m3 !! i).
+    Qed.
 
-  Definition hprop := heap -> Prop.
+    Definition heap_union_comm (h1 h2 : heap) := map_union_comm h1 h2.
+
+    Lemma heap_disjoint_union_l_l : forall (h1 h2 h3 :heap) , h1 ∪ h2 ##ₘ h3 -> h1 ##ₘ h3.
+    Proof.
+      intros. apply map_disjoint_union_l in H as (P0&P1). assumption.
+    Qed.
+
+    Lemma heap_disjoint_union_l_r : forall (h1 h2 h3 :heap) , h1 ∪ h2 ##ₘ h3 -> h2 ##ₘ h3.
+    Proof.
+      intros. apply map_disjoint_union_l in H as (P0&P1). assumption.
+    Qed.
+
+    Lemma heap_disjoint_union_r_r : forall (h1 h2 h3 :heap) , h1 ##ₘ h2 ∪ h3 -> h1 ##ₘ h3.
+    Proof.
+      intros. apply map_disjoint_union_r in H as (P0&P1). assumption.
+    Qed.
+
+    Lemma heap_disjoint_union_r_l : forall (h1 h2 h3 :heap) , h1 ##ₘ h2 ∪ h3 -> h1 ##ₘ h2.
+    Proof.
+      intros. apply map_disjoint_union_r in H as (P0&P1). assumption.
+    Qed.
+
+    (* Operators *)
+
+    Definition hprop := heap -> Prop.
+
+    Definition hand (H1 H2:hprop):hprop :=
+      fun h => H1 h /\ H2 h.
+
+    Definition hor (H1 H2:hprop) : hprop := fun h => H1 h \/ H2 h.
+
+    Definition hempty : hprop :=
+      fun h => h = ∅.
+
+    Definition hsingle loc t : hprop :=
+      fun h =>  h = {[loc := t]}.
+
+    Definition hheap_ctx (ctx : heap) : hprop := fun h => h = ctx.
+
+    Definition hstar (H1 H2 : hprop) : hprop :=
+      fun h => exists h1 h2, H1 h1
+                     /\ H2 h2
+                     /\ (h1 ##ₘ h2)
+                     /\ h = h1 ∪ h2.
+
+    Definition hexists {A} (J : A -> hprop) : hprop :=
+      fun h => exists x, J x h.
+
+    Definition hpure (P:Prop) : hprop :=
+      fun h => P /\ hempty h.
+
+    Definition htop : hprop :=
+      fun h => True.
+
+    Definition hforall {A} (f : A -> hprop) : hprop := fun h => forall a, f a h.
+
+
+    Definition hwand (H1 H2 : hprop) : hprop :=
+      hexists (fun (H:hprop) => (hstar H (hpure ((hstar H H1) ==> H2)))).
+
+    Definition qwand A (Q1 Q2:A->hprop) :=
+      hforall (fun x => hwand (Q1 x) (Q2 x)).
+
+    Definition hpure_abs (φ : Prop) : hprop := hstar (hpure φ) htop.
+
+
+    Lemma hempty_intro : hempty ∅.
+    Proof using. reflexivity. Qed.
+
+    Lemma hempty_inv : forall h, hempty h -> h = ∅.
+    Proof using. auto. Qed.
+
+    Local Notation "'heap_empty'" := (∅ : heap).
+
+    Local Notation "h1 \u h2" := (h1 ∪ h2) (at level 37, right associativity).
+
+    Local Notation "'Hexists' x1 , H" := (hexists (fun x1 => H))
+                                           (at level 39, x1 ident, H at level 50).
+    Local Notation "'Hexists' x1 x2 , H" := (Hexists x1, Hexists x2, H)
+                                              (at level 39, x1 ident, x2 ident, H at level 50).
+    Local Notation "'Hexists' x1 x2 x3 , H" := (Hexists x1, Hexists x2, Hexists x3, H)
+                                                 (at level 39, x1 ident, x2 ident, x3 ident, H at level 50).
+
+
+    Local Notation "'\[]'" := (hempty)
+                                (at level 0).
+
+    Local Notation "\[ P ]" := (hpure P)
+                                 (at level 0, P at level 99, format "\[ P ]").
+
+    Local Notation "H1 '\*' H2" := (hstar H1 H2)
+                                     (at level 41, right associativity).
+
+    Local Notation "\Top" := htop.
+
+
+    Declare Scope heap_scope.
+
+    Hint Resolve heap_union_empty_l heap_union_empty_r hempty_intro map_disjoint_empty_l map_disjoint_empty_r heap_union_assoc heap_disjoint_union_r_l heap_disjoint_union_l_l heap_disjoint_union_r_r heap_disjoint_union_l_r : heap_scope.
+
+    Ltac inversion_star h P :=
+      match goal with
+      | H : (_ \* _) _ |- _ =>
+        let W := fresh h in
+        let w := fresh P in
+        inversion H as (W&w);
+        let W := fresh h in
+        destruct w as (W&w);
+        do 3 (let w0 := fresh P in
+              destruct w as (w0&w))
+      end.
+    Ltac extens := apply functional_extensionality; intro; apply prop_extensionality.
+
+    Section Properties.
+
+      Lemma hstar_intro : forall (H1 H2 :hprop) h1 h2,
+        H1 h1 ->
+        H2 h2 ->
+        h1 ##ₘ h2 ->
+        (H1 \* H2) (h1 ∪ h2).
+      Proof using. intros. exists h1; exists h2. auto. Qed.
+
+      Lemma hstar_hempty_l : forall H,
+          hempty \* H = H.
+      Proof using.
+        intros. extens.
+        split; intro.
+        - inversion_star h P. inversion P0; subst. rewrite heap_union_empty_l. assumption.
+        - exists heap_empty; exists x. repeat split; auto with heap_scope. apply map_disjoint_empty_l.
+      Qed.
+
+      Lemma hstar_comm : forall H1 H2,
+          H1 \* H2 = H2 \* H1.
+      Proof using.
+        intros H1 H2. extens.
+        split; intro P; inversion_star h P; exists h0; exists h; repeat split; auto;
+          rewrite heap_union_comm; auto.
+      Qed.
+
+      Lemma hstar_assoc : forall H1 H2 H3,
+          (H1 \* H2) \* H3 = H1 \* (H2 \* H3).
+      Proof using.
+        intros H1 H2 H3. extens. split.
+        { intros (h'&h3&(h1&h2&M3&M4&D'&U')&M2&D&U). subst h'.
+          exists h1; exists (h2 ∪ h3). repeat split; auto.
+          { exists h2; exists h3; eauto with heap_scope. }
+          { apply map_disjoint_union_l in D as (P0&P1).
+            apply map_disjoint_union_r. split; auto. }
+          { by rewrite heap_union_assoc. }}
+        { intros (h1&h'&M1&(h2&h3&M3&M4&D'&U')&D&U). subst h'.
+          exists (h1 ∪ h2); exists h3. repeat split; auto.
+          { exists h1; exists h2; eauto with heap_scope. }
+          { rewrite map_disjoint_union_l. split; auto.
+            apply map_disjoint_union_r in D as (P0&P1).
+            assumption. }
+            by rewrite <- heap_union_assoc. }
+      Qed.
+
+      Lemma hstar_hexists : forall A (J:A->hprop) H,
+          (hexists J) \* H = hexists (fun x => (J x) \* H).
+      Proof using.
+        intros. extens. split; intro M.
+        { destruct M as (h1&h2&(h3&M1)&M2&D&U). exists h3; exists h1; exists h2; eauto. }
+        { destruct M as (h3&(h1&h2&M1&M2&D&U)). exists h1; exists h2. split; eauto. by exists h3. }
+      Qed.
+
+      Lemma himpl_frame_l : forall H2 H1 H1',
+          H1 ==> H1' ->
+          (H1 \* H2) ==> (H1' \* H2).
+      Proof using. intros. intros h P. inversion_star h P. exists h0; exists h1. split; eauto. Qed.
+
+    End Properties.
+
+    Definition hpersistent (H:hprop) : hprop := fun h => H heap_empty.
+
+    Set Warnings "-redundant-canonical-projection".
+    Canonical Structure hpropO := leibnizO hprop.
+
+    Definition hprop_emp := hpure True.
+
+    Program Canonical Structure hpropI : bi :=
+      Bi hprop _ _ pred_incl hprop_emp hpure_abs hand hor
+         pred_impl (@hforall) (@hexists) hstar hwand hpersistent _ _.
+    Next Obligation.
+      apply discrete_ofe_mixin, _.
+    Qed.
+    Next Obligation.
+      repeat split; try(solve_proper); eauto.
+      - intros H h P. assumption.
+      - rewrite /Transitive. intros. intros h P. eauto.
+      - rewrite leibniz_equiv_iff. intros (P0&P1). extens. split; intro; auto.
+      - intros X Y Z. rewrite /hpure_abs. repeat red. intro. extens.
+        split; intro; inversion_star h P; exists h; exists h0; repeat split; auto; inversion P0; inversion H2;
+          auto with heap_scope; apply H; assumption.
+      - intros X Y Z. rewrite /hforall. repeat red. intros. extens. split; intros; repeat red in H;
+                                                                      apply functional_extensionality in H; subst; auto.
+      - intros X Y Z. rewrite /hexists. repeat red. intros. extens.
+        split; intro; repeat red in H; apply functional_extensionality in H; subst; auto.
+      - rewrite /hpure_abs. intros φ P. exists heap_empty. exists x. repeat split; auto with heap_scope.
+        apply map_disjoint_empty_l.
+      - unfold hpure_abs in *. intros x W P h P0. inversion_star h P. inversion P2. apply P; auto.
+        exists h0; exists h1. repeat split; auto.
+      - rewrite /hforall /hpure_abs. intros h W h0 P. exists heap_empty; exists h0.
+        repeat split; auto with heap_scope.
+        + intro a. pose (P a). inversion_star h P. inversion P1. apply H.
+        + apply map_disjoint_empty_l.
+      - rewrite /hand. intros P Q h (P0&P1). apply P0.
+      - rewrite /hand. intros P Q h (P0&P1). apply P1.
+      - rewrite /hor. intros P Q h P0. auto.
+      - rewrite /hor. intros P Q h P0. auto.
+      - rewrite /hor. intros P Q h P0 P1 h0 P2. destruct P2; auto.
+      - intros x W X H h P x0. apply H. split; auto.
+      - intros x W X H h P. destruct P. apply H in H0. apply H0 in H1. assumption.
+      - intros x W a H h P h0. apply H. apply P.
+      - intros h Q a H H0. apply H0.
+      - intros x W H P Q. exists H. apply Q.
+      - intros x W Q P h P0. destruct P0. eapply P. apply H.
+      - intros P P' Q Q' A B C D. inversion_star h P. exists h; exists h0. repeat split; auto.
+      - intros x W A. exists heap_empty; exists W. repeat split; auto with heap_scope.
+        apply map_disjoint_empty_l.
+      - intros P h Q. inversion_star H H. inversion H3; inversion H6; subst.
+        rewrite heap_union_empty_l. apply H4.
+      - intros P Q h R. inversion_star H H. exists H2; exists H0. repeat split; auto. subst.
+        apply heap_union_comm. apply H5.
+      - intros P Q R h P0. rewrite <- hstar_assoc. apply P0.
+      - intros P Q R P0 h P1. exists P. exists h; exists heap_empty. repeat split; auto with heap_scope.
+        apply map_disjoint_empty_r.
+      - intros P Q R W h P0. inversion_star h P. apply W in P2. destruct P2. inversion_star h H.
+        inversion H2. apply H4. exists h2; exists h1. repeat split; auto; subst.
+        + apply heap_disjoint_union_l_l in P4. apply P4.
+        + inversion H5. subst. rewrite heap_union_empty_r. reflexivity.
+      - rewrite /hpersistent. intros P Q H h P0. apply H. apply P0.
+      - rewrite /hpersistent. rewrite /hforall. intros A B C D E. apply D.
+      - rewrite /hpersistent. intros P Q h P0. inversion_star h P. apply P2.
+      - intros P Q x W. destruct W. exists heap_empty; exists x. repeat split; auto with heap_scope.
+        apply map_disjoint_empty_l.
+    Qed.
+
+
+    Lemma hpure_pure φ : \[φ] = bi_affinely ⌜φ⌝.
+    Proof.
+      extens. split.
+      - intro. destruct H. split. split; auto. exists heap_empty; exists x. repeat split; auto with heap_scope.
+        apply map_disjoint_empty_l.
+      - intros [? Hφ]. destruct Hφ as (h1&h2&P0&P1&P2&P3). destruct P0. repeat split; auto.
+        inversion H. apply H3.
+    Qed.
+
+    Lemma htop_True : \Top = True%I.
+    Proof.
+      extens. split.
+      - exists heap_empty; exists x. repeat split; auto with heap_scope. apply map_disjoint_empty_l.
+      - red; trivial.
+    Qed.
+
+    Opaque hpure_abs.
+
+    (** * Specific Proofmode instances about hpure and htop. *)
+
+    Global Instance htop_absorbing : Absorbing \Top.
+    Proof. intros ??. red; trivial. Qed.
+    Global Instance htop_persistent : Persistent \Top.
+    Proof. intros ??. repeat red. trivial. Qed.
+
+    Global Instance htop_into_pure : IntoPure \Top True.
+    Proof.
+      unfold IntoPure. intros h H. exists ∅, h. repeat split; auto with heap_scope.
+      apply map_disjoint_empty_l.
+    Qed.
+    Global Instance htop_from_pure a : FromPure a \Top True.
+    Proof. intros ??. red; trivial. Qed.
+
+    Global Instance hpure_affine φ : Affine \[φ].
+    Proof. rewrite hpure_pure. apply _. Qed.
+    Global Instance hpure_persistent φ : Persistent \[φ].
+    Proof. rewrite hpure_pure. apply _. Qed.
+
+    Global Instance hpure_into_pure φ : IntoPure \[φ] φ.
+    Proof. rewrite hpure_pure /IntoPure. intros h H. destruct H. auto. Qed.
+    Global Instance hpure_from_pure φ : FromPure true \[φ] φ.
+    Proof. by rewrite hpure_pure /FromPure /= /bi_affinely stdpp.base.comm. Qed.
+
+    Global Instance from_and_hpure φ ψ : FromAnd \[φ ∧ ψ] \[φ] \[ψ].
+    Proof.
+      rewrite /FromAnd. intros h H. destruct H. inversion H. inversion H0. repeat eexists; auto.
+    Qed.
+    Global Instance from_sep_hpure φ ψ : FromSep \[φ ∧ ψ] \[φ] \[ψ].
+    Proof.
+      rewrite /FromSep. intros h H. red in H. inversion_star h P.
+      inversion P0. inversion P1. inversion H1. inversion H3. subst. rewrite heap_union_empty_l.
+      repeat eexists; auto.
+    Qed.
+
+
+
+    Global Instance into_and_hpure (p : bool) φ ψ : IntoAnd p \[φ ∧ ψ] \[φ] \[ψ].
+    Proof. rewrite /IntoAnd. f_equiv. auto. Qed.
+    Global Instance into_sep_hpure φ ψ : IntoSep \[φ ∧ ψ] \[φ] \[ψ].
+    Proof. rewrite /IntoSep. auto. Qed.
+    Global Instance from_or_hpure φ ψ : FromOr \[φ ∨ ψ] \[φ] \[ψ].
+    Proof. rewrite /FromOr. auto. Qed.
+    Global Instance into_or_hpure φ ψ : IntoOr \[φ ∨ ψ] \[φ] \[ψ].
+    Proof. rewrite /IntoOr. auto. Qed.
+    Global Instance from_exist_hpure {A} (φ : A → Prop) :
+      FromExist \[∃ x : A, φ x] (λ a : A, \[φ a]).
+    Proof. rewrite /FromExist. auto. Qed.
+    Global Instance into_exist_hpure {A} (φ : A → Prop) :
+      IntoExist \[∃ x : A, φ x] (λ a : A, \[φ a]).
+    Proof. rewrite /IntoExist. auto. Qed.
+    Global Instance from_forall_hpure {A : Type} `{Inhabited A} (φ : A → Prop) :
+      FromForall \[∀ a : A, φ a] (λ a : A, \[φ a]).
+    Proof. rewrite /FromForall. auto. Qed.
+    Global Instance frame_here_hpure p (φ : Prop) Q :
+      FromPure true Q φ → Frame p \[φ] Q emp.
+    Proof.
+      rewrite /FromPure /Frame=><- /=. destruct p=>/=; iIntros "[% _] !%"; auto.
+    Qed.
+
+    (** Instance affine *)
+
+    Global Instance from_affinely_affine P : Affine P → @FromAffinely hpropI P P.
+    Proof. intros. rewrite /FromAffinely. iIntros "HA". iApply "HA". Qed.
+    Global Instance from_affinely_default P : @FromAffinely hpropI (<affine> P) P | 100.
+    Proof. by rewrite /FromAffinely. Qed.
+    Global Instance from_affinely_intuitionistically P : @FromAffinely hpropI (□ P) (<pers> P) | 100.
+    Proof. by rewrite /FromAffinely. Qed.
+
+    (** Instance Sep *)
+
+    Global Instance from_sep_sep P1 P2 : @FromSep hpropI (P1 ∗ P2) P1 P2 | 100.
+    Proof. by rewrite /FromSep. Qed.
+
+    Global Instance into_sep_sep P Q : @IntoSep hpropI (P ∗ Q) P Q.
+    Proof. by rewrite /IntoSep. Qed.
+
+    (** Instance Wand *)
+
+    Global Instance from_wand_wand P1 P2 : @FromWand hpropI (P1 -∗ P2) P1 P2.
+    Proof. by rewrite /FromWand. Qed.
+
+
+    Instance inhabited_unit : Inhabited unit.
+    Proof.
+      split. apply ().
+    Qed.
+
+    Instance PreOrder_unit : PreOrder (fun (t1 t2 : unit) => t1 = t2).
+    Proof.
+      split; repeat red; intros; trivial. destruct x,y,z. reflexivity.
+    Qed.
+
+    Program Canonical Structure biInd := BiIndex unit inhabited_unit _ PreOrder_unit.
+
+    Definition single (l : positive) (t : type) : monPred biInd hpropI := MonPred (fun _ => hsingle l t) _.
+
+    Definition heap_ctx (h : heap) : monPred biInd hpropI := MonPred (fun _ => hheap_ctx h) _.
+
+    Ltac inv H := inversion H; clear H; subst.
+
+    Lemma test : forall l, ⊢ (∃ t, single l t) -∗ (∃ t, single l t) -∗ False.
+    Proof.
+      MonPred.unseal. split. MonPred.unseal. repeat red. intros. destruct i. destruct a. clear H0.
+      inv H. inv H1. clear H0. exists hempty, heap_empty, heap_empty. repeat split; auto with heap_scope.
+      intros h H j C. clear C. clear j. inversion_star h P. clear H. inv P0. clear P2.
+      destruct P1. red in H. rewrite heap_union_empty_l. exists (hheap_ctx h1), h1, heap_empty.
+      repeat split; eauto with heap_scope. subst. intros h H. inversion_star h P. destruct P1.
+      red in H0. red in P0. subst. clear H. erewrite map_disjoint_spec in P2.
+      edestruct P2; eapply lookup_singleton_Some; eauto.
+      apply map_disjoint_empty_r.
+    Qed.
+
+    Local Open Scope bi_scope.
+    Local Notation "l ↦ t" :=
+      (single l t) (at level 20) : bi_scope.
+
+    Local Notation "\s l" :=
+      (∃ t, l ↦ t) (at level 10) : bi_scope.
+
+    Lemma singleton_false : forall t, ⊢ \s t -∗ \s t -∗ False.
+    Proof.
+      MonPred.unseal. split. MonPred.unseal. repeat red. intros. destruct i. destruct a. clear H0.
+      inv H. inv H1. clear H0. exists emp, heap_empty, heap_empty. repeat split; auto with heap_scope.
+      intros h H j C. clear C. clear j. inversion_star h P. clear H. inv P0. inv H0. clear H. clear P2.
+      destruct P1. red in H. rewrite heap_union_empty_l. exists (hheap_ctx h1), h1, heap_empty.
+      repeat split; eauto with heap_scope. subst. intros h H. inversion_star h P. destruct P1.
+      red in H0. red in P0. subst. clear H. erewrite map_disjoint_spec in P2.
+      edestruct P2; eapply lookup_singleton_Some; eauto.
+      apply map_disjoint_empty_r.
+    Qed.
+
+
+  End hprop.
+
+  (* Arguments hand [type]. *)
+  (* Arguments hor [type]. *)
+  (* Arguments hempty [type]. *)
+  (* Arguments hsingle [type]. *)
+  (* Arguments hheap_ctx [type]. *)
+  (* Arguments hstar [type]. *)
+  (* Arguments hexists [type]. *)
+  (* Arguments hpure [type]. *)
+  (* Arguments htop [type]. *)
+  (* Arguments hforall [type]. *)
+  (* Arguments hwand [type]. *)
+  (* Arguments qwand [type]. *)
+
+
+  (* Arguments hstar [type]. *)
+
+  (* Arguments heap_ctx [type]. *)
 
   Notation "'heap_empty'" := (∅ : heap).
 
   Notation "h1 \u h2" := (h1 ∪ h2) (at level 37, right associativity).
-
-  (* Properties on heap *)
-  Instance heap_union_empty_l : LeftId (=@{heap}) ∅ (∪) := _.
-  Instance heap_union_empty_r : RightId (=@{heap}) ∅ (∪) := _.
-  Instance heap_union_assoc : base.Assoc (=@{heap}) (∪).
-  Proof.
-    intros m1 m2 m3. unfold base.union, map_union, union_with, map_union_with.
-    apply (merge_assoc _). intros i.
-    unfold heap in m1. unfold heap in m2. unfold heap in m3.
-      by destruct (m1 !! i), (m2 !! i), (m3 !! i).
-  Qed.
-
-  Definition heap_union_comm (h1 h2 : heap) := map_union_comm h1 h2.
-
-  Lemma heap_disjoint_union_l_l : forall (h1 h2 h3 :heap) , h1 ∪ h2 ##ₘ h3 -> h1 ##ₘ h3.
-  Proof.
-    intros. apply map_disjoint_union_l in H as (P0&P1). assumption.
-  Qed.
-
-  Lemma heap_disjoint_union_l_r : forall (h1 h2 h3 :heap) , h1 ∪ h2 ##ₘ h3 -> h2 ##ₘ h3.
-  Proof.
-    intros. apply map_disjoint_union_l in H as (P0&P1). assumption.
-  Qed.
-
-  Lemma heap_disjoint_union_r_r : forall (h1 h2 h3 :heap) , h1 ##ₘ h2 ∪ h3 -> h1 ##ₘ h3.
-  Proof.
-    intros. apply map_disjoint_union_r in H as (P0&P1). assumption.
-  Qed.
-
-  Lemma heap_disjoint_union_r_l : forall (h1 h2 h3 :heap) , h1 ##ₘ h2 ∪ h3 -> h1 ##ₘ h2.
-  Proof.
-    intros. apply map_disjoint_union_r in H as (P0&P1). assumption.
-  Qed.
-
-  (* Operators *)
-
-  Definition hand (H1 H2:hprop):hprop :=
-    fun h => H1 h /\ H2 h.
-
-  Definition hor (H1 H2:hprop) : hprop := fun h => H1 h \/ H2 h.
-
-  Definition hempty : hprop :=
-    fun h => h = heap_empty.
-
-  Definition hsingle loc t : hprop :=
-    fun h =>  h = {[loc := t]}.
-  
-  Definition hheap_ctx (ctx : heap) : hprop := fun h => h = ctx.
-
-  Definition hstar (H1 H2 : hprop) : hprop :=
-    fun h => exists h1 h2, H1 h1
-                   /\ H2 h2
-                   /\ (h1 ##ₘ h2)
-                   /\ h = h1 ∪ h2.
-
-  Definition hexists {A} (J : A -> hprop) : hprop :=
-    fun h => exists x, J x h.
-
-  Definition hpure (P:Prop) : hprop :=
-    fun h => P /\ hempty h.
-
-  Definition htop : hprop :=
-    fun h => True.
-
-  Definition hforall {A} (f : A -> hprop) : hprop := fun h => forall a, f a h.
 
   Notation "'Hexists' x1 , H" := (hexists (fun x1 => H))
                                    (at level 39, x1 ident, H at level 50).
@@ -98,40 +455,18 @@ Module SepBasicCore.
   Notation "'Hexists' x1 x2 x3 , H" := (Hexists x1, Hexists x2, Hexists x3, H)
                                          (at level 39, x1 ident, x2 ident, x3 ident, H at level 50).
 
+  Notation "'\[]'" := (hempty) (at level 0).
 
-  Notation "'\[]'" := (hempty)
-                        (at level 0).
+  Notation "\[ P ]" := (hpure P) (at level 0, P at level 99, format "\[ P ]").
 
-  Notation "\[ P ]" := (hpure P)
-                         (at level 0, P at level 99, format "\[ P ]").
-
-  Notation "H1 '\*' H2" := (hstar H1 H2)
-                             (at level 41, right associativity).
+  Notation "H1 '\*' H2" := (hstar H1 H2) (at level 41, right associativity).
 
   Notation "\Top" := htop.
 
-  Definition hwand (H1 H2 : hprop) : hprop :=
-    hexists (fun (H:hprop) => H \* (hpure (H \* H1 ==> H2))).
-
-  Definition qwand A (Q1 Q2:A->hprop) :=
-    hforall (fun x => hwand (Q1 x) (Q2 x)).
-
-  Definition hpure_abs (φ : Prop) : hprop := \[φ] \* \Top.
-
-  Lemma hempty_intro :
-    \[] heap_empty.
-  Proof using. reflexivity. Qed.
-
-  Lemma hempty_inv : forall h,
-      \[] h ->
-      h = heap_empty.
-  Proof using. auto. Qed.
-  
   Declare Scope heap_scope.
-  
+
   Hint Resolve heap_union_empty_l heap_union_empty_r hempty_intro map_disjoint_empty_l map_disjoint_empty_r heap_union_assoc heap_disjoint_union_r_l heap_disjoint_union_l_l heap_disjoint_union_r_r heap_disjoint_union_l_r : heap_scope.
 
-  
   Ltac inversion_star h P :=
     match goal with
     | H : (_ \* _) _ |- _ =>
@@ -144,275 +479,23 @@ Module SepBasicCore.
             destruct w as (w0&w))
     end.
 
-  Ltac extens := apply functional_extensionality; intro; apply prop_extensionality.
+  Open Scope bi_scope.
 
-  Section Properties.
-    
-    
+  (* Arguments single [type]. *)
+  (* Arguments heap_ctx [type]. *)
 
-    Lemma hstar_intro : forall (H1 H2 :hprop) h1 h2,
-      H1 h1 ->
-      H2 h2 ->
-      h1 ##ₘ h2 ->
-      (H1 \* H2) (h1 ∪ h2).
-    Proof using. intros. exists h1; exists h2. auto. Qed.
+  Notation "l ↦ t" :=
+    (single l t) (at level 20) : bi_scope.
 
-    Lemma hstar_hempty_l : forall H,
-        hempty \* H = H.
-    Proof using.
-      intros. extens. 
-      split; intro.
-      - inversion_star h P. inversion P0; subst. rewrite heap_union_empty_l. assumption.
-      - exists heap_empty; exists x. repeat split; auto with heap_scope. apply map_disjoint_empty_l.
-    Qed.
+  Notation "\s l" :=
+    (∃ t, l ↦ t) (at level 10) : bi_scope.
 
-    Lemma hstar_comm : forall H1 H2,
-        H1 \* H2 = H2 \* H1.
-    Proof using.
-      intros H1 H2. extens.
-      split; intro P; inversion_star h P; exists h0; exists h; repeat split; auto;
-        rewrite heap_union_comm; auto.
-    Qed.
-
-    Lemma hstar_assoc : forall H1 H2 H3,
-        (H1 \* H2) \* H3 = H1 \* (H2 \* H3).
-    Proof using.
-      intros H1 H2 H3. extens. split.
-      { intros (h'&h3&(h1&h2&M3&M4&D'&U')&M2&D&U). subst h'.
-        exists h1; exists (h2 ∪ h3). repeat split; auto.
-        { exists h2; exists h3; eauto with heap_scope. }
-        { apply map_disjoint_union_l in D as (P0&P1).
-          apply map_disjoint_union_r. split; auto. }
-        { by rewrite heap_union_assoc. }}
-      { intros (h1&h'&M1&(h2&h3&M3&M4&D'&U')&D&U). subst h'.
-        exists (h1 ∪ h2); exists h3. repeat split; auto.
-        { exists h1; exists h2; eauto with heap_scope. }
-        { rewrite map_disjoint_union_l. split; auto.
-          apply map_disjoint_union_r in D as (P0&P1).
-          assumption. }
-          by rewrite <- heap_union_assoc. }
-    Qed.
-
-    Lemma hstar_hexists : forall A (J:A->hprop) H,
-        (hexists J) \* H = hexists (fun x => (J x) \* H).
-    Proof using.
-      intros. extens. split; intro M.
-      { destruct M as (h1&h2&(h3&M1)&M2&D&U). exists h3; exists h1; exists h2; eauto. }
-      { destruct M as (h3&(h1&h2&M1&M2&D&U)). exists h1; exists h2. split; eauto. by exists h3. }
-    Qed.
-
-    Lemma himpl_frame_l : forall H2 H1 H1',
-        H1 ==> H1' ->
-        (H1 \* H2) ==> (H1' \* H2).
-    Proof using. intros. intros h P. inversion_star h P. exists h0; exists h1. split; eauto. Qed.
-
-  End Properties.
-
-  Definition hpersistent (H:hprop) : hprop := fun h => H heap_empty.
 
 End SepBasicCore.
 
-Export SepBasicCore.
-
-Module ProofModeInstantiate.
-  Set Warnings "-redundant-canonical-projection".
-  Canonical Structure hpropO := leibnizO hprop.
-  
-  Definition hprop_emp := hpure True.
-
-  Program Canonical Structure hpropI : bi :=
-    Bi hprop _ _ pred_incl hprop_emp hpure_abs hand hor
-       pred_impl (@hforall) (@hexists) hstar hwand hpersistent _ _.
-  Next Obligation.
-    apply discrete_ofe_mixin, _.
-  Qed.
-  Next Obligation.
-    repeat split; try(solve_proper); eauto.
-    - intros H h P. assumption.
-    - rewrite /Transitive. intros. intros h P. eauto.
-    - rewrite leibniz_equiv_iff. intros (P0&P1). extens. split; intro; auto.
-    - intros X Y Z. rewrite /hpure_abs. repeat red. intro. extens.
-      split; intro; inversion_star h P; exists h; exists h0; repeat split; auto; inversion P0; inversion H2;
-        auto with heap_scope; apply H; assumption.
-    - intros X Y Z. rewrite /hforall. repeat red. intros. extens. split; intros; repeat red in H;
-      apply functional_extensionality in H; subst; auto.
-    - intros X Y Z. rewrite /hexists. repeat red. intros. extens. 
-      split; intro; repeat red in H; apply functional_extensionality in H; subst; auto.
-    - rewrite /hpure_abs. intros φ P. exists heap_empty. exists x. repeat split; auto with heap_scope.
-      apply map_disjoint_empty_l.
-    - unfold hpure_abs in *. intros x W P h P0. inversion_star h P. inversion P2. apply P; auto.
-      exists h0; exists h1. repeat split; auto.
-    - rewrite /hforall /hpure_abs. intros h W h0 P. exists heap_empty; exists h0.
-      repeat split; auto with heap_scope.
-      + intro a. pose (P a). inversion_star h P. inversion P1. apply H.
-      + apply map_disjoint_empty_l.
-    - rewrite /hand. intros P Q h (P0&P1). apply P0.
-    - rewrite /hand. intros P Q h (P0&P1). apply P1.
-    - rewrite /hor. intros P Q h P0. auto.
-    - rewrite /hor. intros P Q h P0. auto.
-    - rewrite /hor. intros P Q h P0 P1 h0 P2. destruct P2; auto.
-    - intros x W X H h P x0. apply H. split; auto.
-    - intros x W X H h P. destruct P. apply H in H0. apply H0 in H1. assumption.
-    - intros x W a H h P h0. apply H. apply P.
-    - intros h Q a H H0. apply H0.
-    - intros x W H P Q. exists H. apply Q.
-    - intros x W Q P h P0. destruct P0. eapply P. apply H.
-    - intros P P' Q Q' A B C D. inversion_star h P. exists h; exists h0. repeat split; auto.
-    - intros x W A. exists heap_empty; exists W. repeat split; auto with heap_scope.
-      apply map_disjoint_empty_l.
-    - intros P h Q. inversion_star H H. inversion H3; inversion H6; subst.
-      rewrite heap_union_empty_l. apply H4.
-    - intros P Q h R. inversion_star H H. exists H2; exists H0. repeat split; auto. subst.
-      apply heap_union_comm. apply H5.
-    - intros P Q R h P0. rewrite <- hstar_assoc. apply P0.
-    - intros P Q R P0 h P1. exists P. exists h; exists heap_empty. repeat split; auto with heap_scope.
-      apply map_disjoint_empty_r.
-    - intros P Q R W h P0. inversion_star h P. apply W in P2. destruct P2. inversion_star h H.
-      inversion H2. apply H4. exists h2; exists h1. repeat split; auto; subst.
-      + apply heap_disjoint_union_l_l in P4. apply P4.
-      + inversion H5. subst. rewrite heap_union_empty_r. reflexivity.
-    - rewrite /hpersistent. intros P Q H h P0. apply H. apply P0.
-    - rewrite /hpersistent. rewrite /hforall. intros A B C D E. apply D.
-    - rewrite /hpersistent. intros P Q h P0. inversion_star h P. apply P2.
-    - intros P Q x W. destruct W. exists heap_empty; exists x. repeat split; auto with heap_scope.
-      apply map_disjoint_empty_l.
-  Qed.
-
-
-  Lemma hpure_pure φ : \[φ] = bi_affinely ⌜φ⌝.
-  Proof.
-    extens. split.
-    - intro. destruct H. split. split; auto. exists heap_empty; exists x. repeat split; auto with heap_scope.
-      apply map_disjoint_empty_l.
-    - intros [? Hφ]. destruct Hφ as (h1&h2&P0&P1&P2&P3). destruct P0. repeat split; auto.
-      inversion H. apply H3.      
-  Qed.
-
-  Lemma htop_True : \Top = True%I.
-  Proof.
-    extens. split.
-    - exists heap_empty; exists x. repeat split; auto with heap_scope. apply map_disjoint_empty_l.
-    - red; trivial.
-  Qed.
-
-  Opaque hpure_abs.
-
-End ProofModeInstantiate.
-
-Module ProofMode.
-
-  Export ProofModeInstantiate.
-
-  (** * Specific Proofmode instances about hpure and htop. *)
-
-  Global Instance htop_absorbing : Absorbing \Top.
-  Proof. intros ??. red; trivial. Qed.
-  Global Instance htop_persistent : Persistent \Top.
-  Proof. intros ??. repeat red. trivial. Qed.
-
-  Global Instance htop_into_pure : IntoPure \Top True.
-  Proof.
-    unfold IntoPure. intros h H. exists ∅, h. repeat split; auto with heap_scope.
-    apply map_disjoint_empty_l.
-  Qed.
-  Global Instance htop_from_pure a : FromPure a \Top True.
-  Proof. intros ??. red; trivial. Qed.
-
-  Global Instance hpure_affine φ : Affine \[φ].
-  Proof. rewrite hpure_pure. apply _. Qed.
-  Global Instance hpure_persistent φ : Persistent \[φ].
-  Proof. rewrite hpure_pure. apply _. Qed.
-
-  Global Instance hpure_into_pure φ : IntoPure \[φ] φ.
-  Proof. rewrite hpure_pure /IntoPure. intros h H. destruct H. auto. Qed.
-  Global Instance hpure_from_pure φ : FromPure true \[φ] φ.
-  Proof. by rewrite hpure_pure /FromPure /= /bi_affinely stdpp.base.comm. Qed.
-
-  Global Instance from_and_hpure φ ψ : FromAnd \[φ ∧ ψ] \[φ] \[ψ].
-  Proof.
-    rewrite /FromAnd. intros h H. destruct H. inversion H. inversion H0. repeat eexists; auto.
-  Qed.
-  Global Instance from_sep_hpure φ ψ : FromSep \[φ ∧ ψ] \[φ] \[ψ].
-  Proof.
-    rewrite /FromSep. intros h H. red in H. inversion_star h P.
-    inversion P0. inversion P1. inversion H1. inversion H3. subst. rewrite heap_union_empty_l.
-    repeat eexists; auto. 
-  Qed.
-  
-  
-  
-  Global Instance into_and_hpure (p : bool) φ ψ : IntoAnd p \[φ ∧ ψ] \[φ] \[ψ].
-  Proof. rewrite /IntoAnd. f_equiv. auto. Qed.
-  Global Instance into_sep_hpure φ ψ : IntoSep \[φ ∧ ψ] \[φ] \[ψ].
-  Proof. rewrite /IntoSep. auto. Qed.
-  Global Instance from_or_hpure φ ψ : FromOr \[φ ∨ ψ] \[φ] \[ψ].
-  Proof. rewrite /FromOr. auto. Qed.
-  Global Instance into_or_hpure φ ψ : IntoOr \[φ ∨ ψ] \[φ] \[ψ].
-  Proof. rewrite /IntoOr. auto. Qed.
-  Global Instance from_exist_hpure {A} (φ : A → Prop) :
-    FromExist \[∃ x : A, φ x] (λ a : A, \[φ a]).
-  Proof. rewrite /FromExist. auto. Qed.
-  Global Instance into_exist_hpure {A} (φ : A → Prop) :
-    IntoExist \[∃ x : A, φ x] (λ a : A, \[φ a]).
-  Proof. rewrite /IntoExist. auto. Qed.
-  Global Instance from_forall_hpure {A : Type} `{Inhabited A} (φ : A → Prop) :
-    FromForall \[∀ a : A, φ a] (λ a : A, \[φ a]).
-  Proof. rewrite /FromForall. auto. Qed.
-  Global Instance frame_here_hpure p (φ : Prop) Q :
-    FromPure true Q φ → Frame p \[φ] Q emp.
-  Proof.
-    rewrite /FromPure /Frame=><- /=. destruct p=>/=; iIntros "[% _] !%"; auto.
-  Qed.
-
-  (** Instance affine *)
-
-  Global Instance from_affinely_affine P : Affine P → @FromAffinely hpropI P P.
-  Proof. intros. rewrite /FromAffinely. iIntros "HA". iApply "HA". Qed.
-  Global Instance from_affinely_default P : @FromAffinely hpropI (<affine> P) P | 100.
-  Proof. by rewrite /FromAffinely. Qed.
-  Global Instance from_affinely_intuitionistically P : @FromAffinely hpropI (□ P) (<pers> P) | 100.
-  Proof. by rewrite /FromAffinely. Qed.
-
-  (** Instance Sep *)
-
-  Global Instance from_sep_sep P1 P2 : @FromSep hpropI (P1 ∗ P2) P1 P2 | 100.
-  Proof. by rewrite /FromSep. Qed.
-
-  Global Instance into_sep_sep P Q : @IntoSep hpropI (P ∗ Q) P Q.
-  Proof. by rewrite /IntoSep. Qed.
-
-  (** Instance Wand *)
-
-  Global Instance from_wand_wand P1 P2 : @FromWand hpropI (P1 -∗ P2) P1 P2.
-  Proof. by rewrite /FromWand. Qed.                                         
-  
-End ProofMode.
-
-Module biInd.
-  Import ProofMode.
-  Import monpred.
-
-  Instance inhabited_unit : Inhabited unit.
-  Proof.
-    split. apply ().
-  Qed.
-
-  Instance PreOrder_unit : PreOrder (fun (t1 t2 : unit) => t1 = t2).
-  Proof.
-    split; repeat red; intros; trivial. destruct x,y,z. reflexivity.
-  Qed.
-
-  Program Canonical Structure biInd := BiIndex unit inhabited_unit _ PreOrder_unit.
-
-End biInd.
-
-
-
-Module gensym.
+Module fresh.
 
   Definition ident := positive.
-
-  Definition state := heap.
 
   Definition max := Pos.max.
   Definition upper := fun r i => max (i+1) r.
@@ -487,10 +570,12 @@ Module gensym.
           omega.
   Qed.
 
-  Definition fresh_ident (s:state) :=
-    fresh (map_to_list s).*1.
 
-  Lemma fresh_ident_spec : forall (s : state), s !! (fresh_ident s) = None.
+  Import SepBasicCore.
+
+  Definition fresh_ident {A} (s: @heap A) := fresh (map_to_list s).*1.
+
+  Lemma fresh_ident_spec {A} : forall (s : @heap A), s !! (fresh_ident s) = None.
   Proof.
     intros. unfold fresh_ident. pose (fresh_is_fresh (map_to_list s).*1).
     apply not_elem_of_list_to_map in n.
@@ -498,6 +583,91 @@ Module gensym.
     apply n.
   Qed.
 
+End fresh.
+
+(* Module mwp_gen. *)
+(*   (* Context {type : Type}. *) *)
+  
+(*   Record Signature (I : Type): Type := *)
+(*     { Operations: I → Type; *)
+(*       Arities: forall i: I, Operations i → Type; *)
+(*       Sorts: forall i: I, forall op: Operations i, Arities i op → I }. *)
+  
+(*   Arguments Operations [_] _ i. *)
+(*   Arguments Arities [_] _ [_] op. *)
+(*   Arguments Sorts [_] _ [_] [_] ar. *)
+
+(*   Definition Functor {I} (S: Signature I)(X : I → Type)(i : I): Type := *)
+(*     { op : Operations S i & forall ar : Arities S op, X (Sorts S ar) }. *)
+
+(*   Inductive Kleene {I} (S: Signature I)(p : I → Type) (i : I) := *)
+(*   | ret : p i → Kleene S p i *)
+(*   | op : Functor S (Kleene S p) i → Kleene S p i. *)
+
+(*   Inductive sig {A} (X : A) : Type := *)
+(*   | Err : A -> sig X *)
+(*   | Gensym : A -> (ident -> A) -> sig X. *)
+  
+(*   Definition arities {A} (a : A) (s : sig a) := *)
+(*     match s with *)
+(*     | Err _ _ => nat *)
+(*     | Gensym _ _ _ => ident *)
+(*     end. *)
+  
+(*   Definition sort {A} (a : A) (s : sig a) (ar : arities a s) := a. *)
+  
+(*   Definition operation {A} : Signature A := {| Operation := sig; *)
+(*                                                Arities := arities; *)
+(*                                                Sorts := sort *)
+(*                                             |}.  *)
+
+(*   Arguments Err [X]. *)
+(*   Arguments Gensym [X]. *)
+
+(*   Inductive mon (X : Type) : Type := *)
+(*   | ret : X -> mon X *)
+(*   | op : sig (mon X) -> mon X. *)
+
+(*   Arguments ret {_} x. *)
+(*   Arguments op {_} s. *)
+
+(*   Fixpoint bind {X Y} (m : mon X) (f : X -> mon Y) : mon Y := *)
+(*     match m with *)
+(*     | ret x => f x *)
+(*     | op (Err e) => op (Err e) *)
+(*     | op (Gensym t g) => op (Gensym t (fun x => bind (g x) f)) *)
+(*     end. *)
+
+(*   Notation "'let!' x ':=' e1 'in' e2" := (bind e1 (fun x => e2)) *)
+(*                                            (x ident, at level 90). *)
+
+(*   Definition error {X} (e : Errors.errmsg) : mon X := op (Err e). *)
+(*   Definition gensym (t : type) : mon ident := op (Gensym t ret). *)
+
+(*   Definition mon := Kleene sig *)
+          
+(*   Fixpoint mwp {X} (e1 : mon X) (Q : X -> iProp) : iProp := *)
+(*     match e1 with *)
+(*     | ret v => Q v *)
+(*     | op (Err e) => True *)
+(*     | op (Gensym _ f) => *)
+(*       ∀ l, \s l -∗ mwp (f l) Q *)
+(*     end. *)
+
+
+  
+(* End mwp_gen. *)
+
+Require Import Ctypes.
+
+
+Module gensym.
+
+  Import SepBasicCore.
+
+  Definition state := @heap type.
+
+  Import fresh.
   Inductive sig (X : Type) : Type :=
   | Err : Errors.errmsg -> sig X
   | Gensym : type -> (ident -> X) -> sig X.
@@ -552,7 +722,7 @@ Module gensym.
   Inductive err (X: Type) : Type :=
   | Erro : Errors.errmsg -> err X
   | Res : X -> err X.
-  
+
   Arguments Erro [X].
   Arguments Res [X].
   Local Open Scope positive_scope.
@@ -571,31 +741,23 @@ End gensym.
 
 
 Module weakestpre_gensym.
-  Export gensym.
-  Export ProofMode.
   Export proofmode.monpred.
-  Import biInd.
+  Export gensym.
+  Export SepBasicCore.
   Import reduction.
-  
-  Open Scope bi_scope.
-  
-  Definition iProp := monPred biInd hpropI.
 
-  Definition single (l : positive) (t : type) : iProp := MonPred (fun _ => hsingle l t) _.
+  Definition iProp := monPred biInd (@hpropI type).
 
-  Definition heap_ctx (h : heap) : iProp := MonPred (fun _ => hheap_ctx h) _. 
-
-  Global Instance affine_heap_empty : Affine (heap_ctx ∅).
+  Global Instance affine_heap_empty : Affine (heap_ctx ∅ : iProp).
   Proof.
     split. intro. MonPred.unseal. repeat red. intros. split; auto.
   Qed.
 
-  Lemma init_heap : bi_emp_valid (heap_ctx ∅).
+  Lemma init_heap : ⊢ (heap_ctx ∅ : iProp).
   Proof.
-    split. MonPred.unseal. repeat red. intros. inversion H. inversion H1.
-    reflexivity.
+    split. MonPred.unseal. repeat red. intros. inversion H. inversion H1. reflexivity.
   Qed.
-    
+
   Definition pure_empty (P : Prop) : iProp := <affine> ⌜P⌝.
 
   Global Instance affine_pure (P : Prop) : Affine (pure_empty P).
@@ -611,24 +773,6 @@ Module weakestpre_gensym.
 
   Notation "\⌜ P ⌝" := (pure_empty P)
                          (at level 0, P at level 99, format "\⌜ P ⌝").
-  
-  Notation "l ↦ t" :=
-    (single l t) (at level 20) : bi_scope.
-  Notation "\s l" := (∃ t, l ↦ t) (at level 10).
-
-  Ltac inv H := inversion H; clear H; subst.
-  
-  Lemma singleton_false : forall t, ⊢ \s t -∗ \s t -∗ False.
-  Proof.
-    MonPred.unseal. split. MonPred.unseal. repeat red. intros. destruct i. destruct a. clear H0.
-    inv H. inv H1. clear H0. exists emp, heap_empty, heap_empty. repeat split; auto with heap_scope.
-    intros h H j C. clear C. clear j. inversion_star h P. clear H. inv P0. inv H0. clear H. clear P2.
-    destruct P1. red in H. rewrite heap_union_empty_l. exists (hheap_ctx h1), h1, heap_empty.
-    repeat split; eauto with heap_scope. subst. intros h H. inversion_star h P. destruct P1.
-    red in H0. red in P0. subst. clear H. erewrite map_disjoint_spec in P2.
-    edestruct P2; eapply lookup_singleton_Some; eauto.
-    apply map_disjoint_empty_r.
-  Qed.  
 
   Fixpoint mwp {X} (e1 : mon X) (Q : X -> iProp) : iProp :=
     match e1 with
@@ -636,9 +780,9 @@ Module weakestpre_gensym.
     | op (Err e) => True
     | op (Gensym _ f) =>
       ∀ l, \s l -∗ mwp (f l) Q
-    end%I.
+    end.
 
-  
+
   Notation "'WP' e |{ Φ } |" := (mwp e Φ)
                                   (at level 20, e, Φ at level 200, only parsing) : bi_scope.
 
@@ -646,17 +790,18 @@ Module weakestpre_gensym.
                                       (at level 20, e, Q at level 200,
                                        format "'[' 'WP'  e  '[ ' |{  v ,  Q  } | ']' ']'") : bi_scope.
 
+
   Notation "'{{' P } } e {{ x .. y , 'RET' pat ; Q } }" :=
     (∀ Φ,
         P -∗ (∀ x, .. (∀ y, Q -∗ Φ pat) .. ) -∗ WP e |{ Φ }|)%I
                                                              (at level 20, x closed binder, y closed binder,
                                                               format "'[hv' {{  P  } }  '/  ' e  '/'  {{  x  ..  y ,  RET  pat ;  Q  } } ']'") : bi_scope.
-  
+
   (** wp rules *)
   (** Generic rules *)
   Lemma wp_value' {X} (Φ : X -> iProp) (v : X) : Φ v ⊢ WP ret v |{ Φ }|%I.
   Proof. auto. Qed.
-  
+
   Lemma wp_value_inv' {X} Φ (v : X) : WP ret v |{ Φ }| ⊢ Φ v%I.
   Proof. auto. Qed.
 
@@ -685,13 +830,13 @@ Module weakestpre_gensym.
         iDestruct ("HA" with "HC") as "HA".
         iPoseProof "HB" as "HB". apply e. }}
   Qed.
-  
+
   (** Monad rules *)
   Lemma wp_gensym (t : type) : ⊢ WP gensym t |{ l, \s l }|.
   Proof.
     simpl. iIntros. auto.
   Qed.
-  
+
   Lemma wp_frame_l {X} (e : mon X) Φ (R : iProp) : R ∗ WP e |{ Φ }| ⊢ WP e |{ v, R ∗ Φ v }|.
   Proof. iIntros "[HA HB]". iApply (wp_mono with "HB"). auto with iFrame. Qed.
   Lemma wp_frame_r {X} (e : mon X) Φ R : WP e |{ Φ }| ∗ R ⊢ WP e |{ v, Φ v ∗ R }|.
@@ -710,20 +855,20 @@ Module weakestpre_gensym.
   Lemma ret_spec {X} (v : X) :
     ⊢{{ emp }} ret v {{ v', RET v'; ⌜ v' = v ⌝  }}.
   Proof. iIntros (?) "HA HB". iApply "HB". auto. Qed.
-  
-  
+
+
   Lemma ret_spec_pure {X} (v : X) :
     ⊢{{ emp }} ret v {{ v', RET v'; \⌜ v' = v ⌝  }}.
   Proof.
     iIntros (?) "HA HB". iApply "HB". auto.
   Qed.
-  
+
   Lemma ret_spec_bis {X} (v : X) (Q : X -> iProp) :
     Q v ⊢{{ emp }} ret v {{ v', RET v'; Q v' }}.
   Proof.
     iIntros "HA" (?) "_ HB". iApply "HB". iFrame.
   Qed.
-  
+
   Lemma bind_spec {X Y} (e : mon X) (f : X -> mon Y) Φ' Φ'' H :
     (⊢{{ H }} e {{ v, RET v; Φ'' v }}) ->
     (∀ v, ⊢ {{ Φ'' v }} (f v) {{ v', RET v'; Φ' v' }}) ->
@@ -787,7 +932,7 @@ Module weakestpre_gensym.
   Proof.
     intro P. iIntros (?) "HA HB". iApply (P with "[HA]").
     iFrame.
-    iIntros (v) "HA". iApply "HB". iFrame. 
+    iIntros (v) "HA". iApply "HB". iFrame.
   Qed.
 
   Lemma intro_true_r {X} H Φ' (e : mon X) :
@@ -796,7 +941,7 @@ Module weakestpre_gensym.
   Proof.
     intro P. iIntros (?) "HA HB". iApply (P with "[HA]").
     iFrame.
-    iIntros (v) "HA". iApply "HB". iFrame. 
+    iIntros (v) "HA". iApply "HB". iFrame.
   Qed.
 
 
@@ -808,7 +953,7 @@ Module weakestpre_gensym.
     iIntros. iFrame.
   Qed.
 
-  
+
   Lemma assoc_pre {X} H R Q Φ' (e : mon X):
     (⊢{{ H ∗ R ∗ Q }} e {{ v, RET v; Φ' v }}) <->
     ⊢{{ (H ∗ R) ∗ Q}} e {{ v, RET v; Φ' v }}.
@@ -823,21 +968,21 @@ Module weakestpre_gensym.
     split; iIntros (? ?) "HA HB"; iApply (H0 with "HA"); iIntros (?) "[HA HC]"; iApply "HB"; iFrame.
     iApply "HC".
   Qed.
-  
+
   Lemma comm_pre {X} H R Φ' (e : mon X):
     (⊢{{ H ∗ R }} e {{ v, RET v; Φ' v }}) <->
     ⊢{{ R ∗ H }} e {{ v, RET v; Φ' v }}.
   Proof.
     split; iIntros (? ?) "[HA HC] HB"; iApply (H0 with "[HA HC]"); iFrame.
   Qed.
-  
+
   Lemma comm_post {X} P H R (e : mon X):
     (⊢{{ P }} e {{ v, RET v; H v ∗ R v }}) <->
     ⊢{{ P }} e {{ v, RET v; R v ∗ H v }}.
   Proof.
     split; iIntros (? ?) "HA HB"; iApply (H0 with "HA"); iIntros (?) "[HA HC]"; iApply "HB"; iFrame.
   Qed.
-  
+
   Lemma forall_useless_post {X Y} P Q (e : mon X):
     (⊢{{ P }} e {{ v, RET v; Q v }}) ->
     ⊢{{ P }} e {{ v, RET v; ∀ (t : Y), Q v }}.
@@ -866,8 +1011,8 @@ Module weakestpre_gensym.
   Proof.
     iIntros (? ?) "[HA HC] HB". iApply (H0 with "[HA HC]"); eauto. iFrame. iApply "HA". trivial.
   Qed.
- 
-  
+
+
   Lemma wand_true_pre_r {X} P H (Q : X -> iProp) e :
     (⊢{{ P ∗ H }} e {{ v, RET v; Q v }}) ->
     ⊢{{ P ∗ (\⌜True⌝ -∗ H) }} e {{ v, RET v; Q v }}.
@@ -875,21 +1020,21 @@ Module weakestpre_gensym.
     iIntros (? ?) "[HA HC] HB". iApply (H0 with "[HA HC]"); eauto. iFrame. iApply "HC". trivial.
   Qed.
 
-  
+
   Lemma wand_true_post_l {X} P H (Q : X -> iProp) e :
     (⊢{{ P }} e {{ v, RET v; Q v ∗ H v }}) ->
     ⊢{{ P }} e {{ v, RET v; (\⌜True⌝ -∗ Q v) ∗ H v }}.
   Proof.
     iIntros (? ?) "HA HB". iApply (H0 with "HA"). iIntros (v) "[HA HC]". iApply "HB". iFrame. eauto.
   Qed.
-  
+
   Lemma wand_true_post_r {X} P H (Q : X -> iProp) e :
     (⊢{{ P }} e {{ v, RET v; Q v ∗ H v }}) ->
     ⊢{{ P }} e {{ v, RET v; Q v ∗ (\⌜True⌝ -∗ H v) }}.
   Proof.
     iIntros (? ?) "HA HB". iApply (H0 with "HA"). iIntros (v) "[HA HC]". iApply "HB". iFrame. eauto.
   Qed.
-  
+
   Lemma forall_wand_true_pre {X Y} P (Q : X -> iProp) e :
     (⊢{{ ∀ (y : Y), P y }} e {{ v, RET v; Q v }}) ->
     ⊢{{ ∀ (y : Y), \⌜True⌝ -∗ P y }} e {{ v, RET v; Q v }}.
@@ -900,8 +1045,8 @@ Module weakestpre_gensym.
   Ltac frameL := apply intro_true_l; apply frame_l.
   Ltac frameR := apply intro_true_r; apply frame_r.
 
-  
-  
+
+
   (** Monad rules *)
   Lemma gensym_spec t :
     ⊢{{ emp }} gensym t {{ l, RET l; \s l }}.
@@ -909,7 +1054,7 @@ Module weakestpre_gensym.
     iIntros (Φ) "HA HB". simpl.
     iIntros (σ) "HC". iApply "HB". iApply "HC".
   Qed.
-  
+
   Lemma error_spec {X} (Q : X -> iProp) e :
     ⊢{{ emp }} error e {{ v, RET v; Q v }}.
   Proof.
@@ -924,20 +1069,20 @@ Module weakestpre_gensym.
     match x with
     | IAnon ?x =>
       let x := eval compute in (ascii_of_pos (x + 64)) in
-      let x := eval compute in (append "H" (string_of_list_ascii [x])) in
-      let env := iGetCtx in
-      let P := reduction.pm_eval (@envs_lookup (monPredI biInd hpropI) x env) in
-      match P with
-      | None => x
-      | Some _ => Fresh
-      end
+          let x := eval compute in (append "H" (string_of_list_ascii [x])) in
+              let env := iGetCtx in
+              let P := reduction.pm_eval (envs_lookup x env) in
+              match P with
+              | None => x
+              | Some _ => Fresh
+              end
     | _ => fail "iFresh returns " x " sometimes."
     end.
-  
+
   (*h should be in the environment *)
   Local Ltac norm h :=
     let env := iGetCtx in
-    let P := reduction.pm_eval (@envs_lookup (monPredI biInd hpropI) h env) in
+    let P := reduction.pm_eval (envs_lookup h env) in
     match P with
     | None => fail "assert false"
     | Some (false, ?P) =>
@@ -963,13 +1108,13 @@ Module weakestpre_gensym.
       | bi_absorbingly _ =>
         let name := Fresh in
         let name_mod := eval compute in (append ">" name) in
-        iPoseProof h as name; iDestruct name as name_mod; norm name
+            iPoseProof h as name; iDestruct name as name_mod; norm name
       | _ =>
         match h with
-        | IAnon _ => 
+        | IAnon _ =>
           let x := Fresh in
           iPoseProof h as x
-        | _ => idtac 
+        | _ => idtac
         end
       end
     | Some (true,?P) => idtac
@@ -987,24 +1132,26 @@ Module weakestpre_gensym.
     iStartProof;
     let env := iGetCtx in
     let list_ident := eval compute in (rev (envs_dom env)) in
-    norm_list list_ident; auto.
+        norm_list list_ident; auto.
 
   Tactic Notation "iNorm" := norm_all.
 
-  Lemma test : forall P Q (R T: iProp), ⊢  <absorb> (T ∗ R) -∗ (∃ (x: nat), (True -∗ T)) -∗ ⌜ P /\ Q ⌝ -∗ ((⌜ P ⌝ -∗ R) ∗ True) -∗ <absorb> R.
+  Lemma test : forall P Q (R T: iProp),
+      ⊢  <absorb> (T ∗ R) -∗ (∃ (x: nat), (True -∗ T)) -∗ ⌜ P /\ Q ⌝ -∗ ((⌜ P ⌝ -∗ R) ∗ True) -∗ <absorb> R.
   Proof. iIntros. destruct a. iNorm. Qed.
-  
+
 End weakestpre_gensym.
 
 Module adequacy.
+  Import fresh.
   Export gensym.
   Export weakestpre_gensym.
 
   Lemma instance_heap : forall (P : iProp) (Q : Prop), (forall tmps, P () tmps -> Q) -> (P ⊢ ⌜Q⌝).
   Proof.
     MonPred.unseal. intros. split. repeat red. intros.
-    exists heap_empty, x. repeat split; auto with heap_scope. destruct i. eapply H. eauto.
-    apply map_disjoint_empty_l.
+    exists ∅, x. repeat split; auto. destruct i. eapply H. eauto.
+    apply map_disjoint_empty_l. rewrite heap_union_empty_l. reflexivity.
   Qed.
 
   Lemma soundness1 h (Φ : Prop) : (heap_ctx h ⊢ (⌜ Φ ⌝) : iProp) -> Φ.
@@ -1015,22 +1162,22 @@ Module adequacy.
     - reflexivity.
     - inversion P0. apply H0.
   Qed.
-  
+
   Lemma soundness2 (Φ : iProp) h : (⊢heap_ctx h -∗ Φ) -> Φ () h.
   Proof.
     MonPred.unseal=> -[H]. repeat red in H.
-    pose (H () heap_empty).
+    pose (H () ∅).
     simpl in *. edestruct e.
     - rewrite monPred_at_emp. split; auto; apply hempty_intro.
-    - repeat red. exists heap_empty; exists heap_empty. repeat split; auto with heap_scope.
+    - repeat red. exists ∅. exists ∅. repeat split; auto. rewrite heap_union_empty_l. auto.
     - inversion_star h P.
       inversion P1.
       apply H1.
       exists heap_empty; exists h.
       inversion H2; subst. rewrite heap_union_empty_r in P; subst.
-      repeat split; auto with heap_scope. apply map_disjoint_empty_l.
+      repeat split; auto. apply map_disjoint_empty_l. rewrite heap_union_empty_l. auto.
   Qed.
-  
+
   Lemma soundness3 (Φ : iProp) h : Φ () h -> (⊢heap_ctx h -∗ Φ).
   Proof.
     MonPred.unseal. unfold monPred_wand_def. unfold monPred_upclosed. simpl. split.
@@ -1038,10 +1185,10 @@ Module adequacy.
     repeat split; auto with heap_scope. rewrite monPred_at_emp in H0. apply H0.
     intros h0 P0. inversion_star h P. simpl in *. rewrite <- P2 in *. inversion P1. inversion H3.
     subst. rewrite heap_union_empty_l. rewrite <- P2. destruct a. apply H.
-    apply map_disjoint_empty_r.
+    apply map_disjoint_empty_r. rewrite heap_union_empty_r. reflexivity.
   Qed.
 
-  Lemma heap_ctx_split h h' : h ##ₘ h' -> (⊢heap_ctx (h \u h') -∗ heap_ctx h ∗ heap_ctx h').
+  Lemma heap_ctx_split (h h' : state) : h ##ₘ h' -> (⊢heap_ctx (h \u h') -∗ heap_ctx h ∗ heap_ctx h').
   Proof.
     intro.
     MonPred.unseal. repeat red.
@@ -1057,13 +1204,13 @@ Module adequacy.
     + inversion H3. rewrite heap_union_empty_l. reflexivity.
   Qed.
 
-  Lemma heap_ctx_split_sing h l t : h ##ₘ ({[l := t]}) ->
-                                    (⊢heap_ctx (<[l := t]>h) -∗ heap_ctx h ∗ l ↦ t).
+  Lemma heap_ctx_split_sing (h : state) l t : h ##ₘ ({[l := t]}) ->
+                                              (⊢heap_ctx (<[l := t]>h) -∗ heap_ctx h ∗ l ↦ t).
   Proof.
     iIntros (?) "HA". rewrite insert_union_singleton_r; auto. iApply heap_ctx_split; auto.
     rewrite <- map_disjoint_singleton_r. eauto.
   Qed.
-  
+
   Lemma adequacy {X} : forall (e : mon X) (Φ : X -> iProp) h v h',
       (heap_ctx h ⊢ WP e |{ Φ }|) ->
       run e h = Res (h', v) ->
@@ -1116,7 +1263,7 @@ Module adequacy.
       iDestruct ("HA" $! (fun v => ⌜ Φ v ⌝) with "HB []") as "HA"; eauto.
     - destruct s.
       + inversion H1.
-      + simpl in H1. eapply e. 
+      + simpl in H1. eapply e.
         2 : apply H1.
         iIntros "HA". pose (fresh_ident_spec h).
         apply (map_disjoint_singleton_r h (fresh_ident h) t) in e0.
@@ -1124,7 +1271,5 @@ Module adequacy.
         iDestruct (H0 with "HA") as "[HA HC]".
         iSplitR "HC". simpl. iIntros (?) "HC HD". iApply ("HA" with "HC [HD]"); eauto. iApply "HC".
   Qed.
-    
+
 End adequacy.
-
-
